work on new specs

verification/theories/memory_tracker/page_allocator/page_allocator_extra.v
@@ -1,6 +1,7 @@
 From refinedrust Require Import typing.
 From ace.theories.page Require Import page_extra.
 
+(*
 (** [m1] is a correct abstraction of [m2] to only specify the number of pages at a given size. *)
 Definition page_allocator_maps_related (m1 : gmap page_size nat) (m2 : gmap page_size (place_rfn (list (place_rfn page)))) : Prop :=
   ∀ (sz : page_size) num_pages, m1 !! sz = Some num_pages →
@@ -11,4 +12,98 @@ Definition page_allocator_maps_related (m1 : gmap page_size nat) (m2 : gmap page
       length list_pages = num_pages ∧
       (* The pages have the right size *)
       Forall (λ pg : page, pg.(page_sz) = sz) list_pages.
+*)
 
+Inductive node_allocation_state :=
+  | PageNodeUnavailable
+  | PageNodeAvailable
+  | PageNodePartiallyAvailable
+.
+
+Global Instance node_allocation_state_eqdec : EqDecision node_allocation_state.
+Proof. solve_decision. Defined.
+
+Search "aligned".
+
+(** Our logical representation of storage nodes *)
+Record page_storage_node : Type := mk_page_node {
+  (* The size of memory this node controls *)
+  max_node_size : page_size;
+  (* The base address of the memory region of this node *)
+  base_address : Z;
+  
+  allocation_state : node_allocation_state;
+}.
+
+(** Compute the base address of a child node *)
+Definition child_base_address (parent_base_address : Z) (child_size : page_size) (child_index : Z) : Z :=
+  parent_base_address + (page_size_in_bytes_Z child_size * child_index).
+
+(** Assert that the base address and node size of the children matches up, that the children are sorted.
+  The list of children need not be complete (i.e. it might also be empty).
+*)
+Definition page_storage_node_children_wf (parent_base_address : Z) (parent_node_size : page_size) (children : list page_storage_node) : Prop :=
+  (* If there is a smaller child node size *)
+  (∀ child_node_size, 
+    page_size_smaller parent_node_size = Some child_node_size →
+    (* Then all children are sorted *)
+    (∀ (i : nat) child, children !! i = Some child → 
+      child.(max_node_size) = child_node_size ∧
+      child.(base_address) = child_base_address parent_base_address parent_node_size i)) ∧
+  (* If there can't be any children, there are no children *)
+  (page_size_smaller parent_node_size = None →
+    children = [])
+.
+
+
+Definition page_storage_node_invariant
+  (node : page_storage_node)
+  (max_sz : option page_size) (maybe_page_token : option page) (children : list page_storage_node) :=
+  (* The children, if any, are well-formed *)
+  page_storage_node_children_wf node.(base_address) node.(max_node_size) children ∧
+  (* the base address is suitably aligned *)
+  (page_size_align node.(max_node_size) | node.(base_address))%Z ∧
+  (* invariant depending on the allocation state: *)
+  if decide (node.(allocation_state) = PageNodeUnavailable) 
+  then 
+      (* No allocation is possible *)
+      maybe_page_token = None ∧ max_sz = None
+  else if decide (node.(allocation_state) = PageNodeAvailable)
+  then
+      (* This node is completely available *) 
+      ∃ token,
+        (* there is some token *)
+        maybe_page_token = Some token ∧
+        (* the token spans the whole node *)
+        token.(page_loc).2 = node.(base_address) ∧
+        token.(page_sz) = node.(max_node_size) ∧
+        (* the allocable size spans the whole page *)
+        max_sz = Some (node.(max_node_size)) ∧
+        (* all children are unavailable *)
+        Forall (λ child, child.(allocation_state) = PageNodeUnavailable) children
+  else 
+      (* This node is partially available with initialized children *)
+      maybe_page_token = None ∧
+      length children = page_size_multiplier node.(max_node_size) ∧
+      (* The maximum size stored in this node needs to be available in one of the children *)
+      ∃ i child, 
+        children !! i = Some child ∧ 
+        child.(allocation_state) = PageNodeAvailable
+.
+
+Lemma page_storage_node_invariant_empty node_size base_address :
+  (page_size_align node_size | base_address) →
+  page_storage_node_invariant (mk_page_node node_size base_address PageNodeUnavailable) None None [].
+Proof.
+  intros.
+  split_and!; simpl; [ | done..].
+  split; done.
+Qed.
+
+
+
+
+Definition page_within_range (base_address : Z) (sz : page_size) (p : page) : Prop :=
+  base_address ≤ p.(page_loc).2 ∧ p.(page_loc).2 + page_size_in_bytes_Z p.(page_sz) < base_address + page_size_in_bytes_Z sz.
+      
+  
